lib/fst/Lib.IntTypes.fst
@@ -15,42 +15,24 @@ let pow2_values n =
     assert_norm (pow2 64 = 0x10000000000000000);
     assert_norm (pow2 128 = 0x100000000000000000000000000000000)
 
-let uint_t (t:inttype) : Type0 =
+let sec_int_t (t:inttype) = pub_int_t t
+
+let sec_int_v #t (u:uint_t t SEC) = pub_int_v #t u
+
+let uintv_extensionality #t #l a b =
   match t with
-  | U8 -> UInt8.t
-  | U16 -> UInt16.t
-  | U32 -> UInt32.t
-  | U64 -> UInt64.t
-  | U128 -> UInt128.t
-  | SIZE -> UInt32.t
-  | BYTE -> UInt8.t
-
-
-inline_for_extraction
-let uint_to_nat_ #t (x:uint_t t) : (n:nat{n <= maxint t}) =
-  match t with
-  | U8 -> UInt8.v x
-  | U16 -> UInt16.v x
-  | U32 -> UInt32.v x
-  | U64 -> UInt64.v x
-  | U128 -> UInt128.v x
-  | SIZE -> UInt32.v x
-  | BYTE -> UInt8.v x
-
-let uint_v #t u : nat = uint_to_nat_ u
-
-let uintv_extensionality #t a b =
-  match t with
+//  | U1   -> admit()
   | U8   -> UInt8.v_inj a b
   | U16  -> UInt16.v_inj a b
   | U32  -> UInt32.v_inj a b
   | U64  -> UInt64.v_inj a b
   | U128 -> UInt128.v_inj a b
-  | SIZE -> UInt32.v_inj a b
-  | BYTE -> UInt8.v_inj a b
+
 
 
 (* Declared in .fsti: uint8, uint16, uint32, uint64, uint128 *)
+
+let secret #t x = x
 
 let u8 x : uint8  = UInt8.uint_to_t x
 
@@ -69,10 +51,10 @@ let u64_uL x = x
 let u128 x : uint128 = UInt128.uint_to_t x
 
 inline_for_extraction
-let size_ x : uint_t SIZE = UInt32.uint_to_t x
+let size_ x : uint_t U32 PUB = UInt32.uint_to_t x
 
 inline_for_extraction
-let byte_ x : uint_t BYTE = UInt8.uint_to_t x
+let byte_ x : uint_t U8 PUB = UInt8.uint_to_t x
 
 inline_for_extraction
 let size x = size_ x
@@ -90,283 +72,251 @@ let size_to_uint32 x = x <: UInt32.t
 
 let byte_to_uint8 x = x <: UInt8.t
 
-let nat_to_uint #t x : uint_t t =
+let nat_to_uint #t #l x : uint_t t l =
   match t with
+//  | U1 -> u8 x
   | U8 -> u8 x
   | U16 -> u16 x
   | U32 -> u32 x
   | U64 -> u64 x
   | U128 -> u128 x
-  | SIZE -> size_ x
-  | BYTE -> byte_ x
+
 
 #reset-options "--z3rlimit 1000 --max_fuel 0"
 #set-options "--lax" // TODO: remove this
-let cast #t t' u  =
+let cast #t #l t' l' u  =
   match t, t' with
   | U8, U8 -> u
   | U8, U16 -> FStar.Int.Cast.uint8_to_uint16 u
   | U8, U32 -> FStar.Int.Cast.uint8_to_uint32 u
-  | U8, SIZE -> FStar.Int.Cast.uint8_to_uint32 u
   | U8, U64 -> FStar.Int.Cast.uint8_to_uint64 u
   | U8, U128 -> FStar.UInt128.uint64_to_uint128 (FStar.Int.Cast.uint8_to_uint64 u)
   | U16, U8 -> FStar.Int.Cast.uint16_to_uint8 u
   | U16, U16 -> u
   | U16, U32 -> FStar.Int.Cast.uint16_to_uint32 u
-  | U16, SIZE -> FStar.Int.Cast.uint16_to_uint32 u
   | U16, U64 -> FStar.Int.Cast.uint16_to_uint64 u
   | U16, U128 -> FStar.UInt128.uint64_to_uint128 (FStar.Int.Cast.uint16_to_uint64 u)
   | U32, U8 -> FStar.Int.Cast.uint32_to_uint8 u
   | U32, U16 -> FStar.Int.Cast.uint32_to_uint16 u
   | U32, U32 -> u
-  | U32, SIZE -> u
   | U32, U64 -> FStar.Int.Cast.uint32_to_uint64 u
   | U32, U128 -> FStar.UInt128.uint64_to_uint128 (FStar.Int.Cast.uint32_to_uint64 u)
-  | SIZE, U8 -> FStar.Int.Cast.uint32_to_uint8 u
-  | SIZE, U16 -> FStar.Int.Cast.uint32_to_uint16 u
-  | SIZE, U32 -> u
-  | SIZE, SIZE -> u
-  | SIZE, U64 -> FStar.Int.Cast.uint32_to_uint64 u
-  | SIZE, U128 -> FStar.UInt128.uint64_to_uint128 (FStar.Int.Cast.uint32_to_uint64 u)
   | U64, U8 -> FStar.Int.Cast.uint64_to_uint8 u
   | U64, U16 -> FStar.Int.Cast.uint64_to_uint16 u
   | U64, U32 -> FStar.Int.Cast.uint64_to_uint32 u
-  | U64, SIZE -> FStar.Int.Cast.uint64_to_uint32 u
   | U64, U64 -> u
   | U64, U128 -> FStar.UInt128.uint64_to_uint128 u
   | U128, U8 -> FStar.Int.Cast.uint64_to_uint8 (FStar.UInt128.uint128_to_uint64 u)
   | U128, U16 -> FStar.Int.Cast.uint64_to_uint16 (FStar.UInt128.uint128_to_uint64 u)
   | U128, U32 -> FStar.Int.Cast.uint64_to_uint32 (FStar.UInt128.uint128_to_uint64 u)
-  | U128, SIZE -> FStar.Int.Cast.uint64_to_uint32 (FStar.UInt128.uint128_to_uint64 u)
   | U128, U64 -> FStar.UInt128.uint128_to_uint64 u
   | U128, U128 -> u
 
 #reset-options "--z3rlimit 100"
 
-let add_mod #t a b =
+let add_mod #t #l a b =
   match t with
+//  | U1  -> admit(); (UInt8.add_mod a b)
   | U8  -> (UInt8.add_mod a b)
   | U16 -> (UInt16.add_mod a b)
   | U32 -> (UInt32.add_mod a b)
   | U64 -> (UInt64.add_mod a b)
   | U128 -> (UInt128.add_mod a b)
-  | SIZE -> (UInt32.add_mod a b)
-  | BYTE -> (UInt8.add_mod a b)
 
-let add #t a b =
+let add #t #l a b =
   match t with
   | U8 -> (UInt8.add a b)
   | U16 -> (UInt16.add a b)
   | U32 -> (UInt32.add a b)
   | U64 -> (UInt64.add a b)
   | U128 -> (UInt128.add a b)
-  | SIZE -> (UInt32.add a b)
-  | BYTE -> (UInt8.add a b)
 
-let incr #t a =
+
+let incr #t #l a =
   match t with
   | U8 -> (UInt8.add a 0x1uy)
   | U16 -> (UInt16.add a 0x1us)
   | U32 -> (UInt32.add a 0x1ul)
   | U64 -> (UInt64.add a 0x1uL)
   | U128 -> (UInt128.add a (UInt128.uint_to_t 1))
-  | SIZE -> (UInt32.add a 0x1ul)
-  | BYTE -> (UInt8.add a 0x1uy)
 
 
-let mul_mod #t a b =
+
+let mul_mod #t #l a b =
   match t with
   | U8 -> (UInt8.mul_mod a b)
   | U16 -> (UInt16.mul_mod a b)
   | U32 -> (UInt32.mul_mod a b)
   | U64 -> (UInt64.mul_mod a b)
-  | SIZE -> (UInt32.mul_mod a b)
-  | BYTE -> (UInt8.mul_mod a b)
 
-let mul #t a b =
+let mul #t #l a b =
   match t with
   | U8 -> (UInt8.mul a b)
   | U16 -> (UInt16.mul a b)
   | U32 -> (UInt32.mul a b)
   | U64 -> (UInt64.mul a b)
-  | SIZE -> (UInt32.mul a b)
-  | BYTE -> (UInt8.mul a b)
 
-let mul_wide a b = UInt128.mul_wide a b
 
-let sub_mod #t a b =
+let mul64_wide a b = UInt128.mul_wide a b
+
+let sub_mod #t #l a b =
   match t with
   | U8 -> (UInt8.sub_mod a b)
   | U16 -> (UInt16.sub_mod a b)
   | U32 -> (UInt32.sub_mod a b)
   | U64 -> (UInt64.sub_mod a b)
   | U128 -> (UInt128.sub_mod a b)
-  | SIZE -> (UInt32.sub_mod a b)
-  | BYTE -> (UInt8.sub_mod a b)
 
-let sub #t a b =
+
+let sub #t #l a b =
   match t with
   | U8 -> (UInt8.sub a b)
   | U16 -> (UInt16.sub a b)
   | U32 -> (UInt32.sub a b)
   | U64 -> (UInt64.sub a b)
   | U128 -> (UInt128.sub a b)
-  | SIZE -> (UInt32.sub a b)
-  | BYTE -> (UInt8.sub a b)
 
-let decr #t a =
+
+let decr #t #l a =
   match t with
   | U8 -> (UInt8.sub a 0x1uy)
   | U16 -> (UInt16.sub a 0x1us)
   | U32 -> (UInt32.sub a 0x1ul)
   | U64 -> (UInt64.sub a 0x1uL)
   | U128 -> (UInt128.sub a (UInt128.uint_to_t 1))
-  | SIZE -> (UInt32.sub a 0x1ul)
-  | BYTE -> (UInt8.sub a 0x1uy)
 
-let logxor #t a b =
+
+let logxor #t #l a b =
   match t with
   | U8 -> (UInt8.logxor a b)
   | U16 -> (UInt16.logxor a b)
   | U32 -> (UInt32.logxor a b)
   | U64 -> (UInt64.logxor a b)
   | U128 -> (UInt128.logxor a b)
-  | SIZE -> (UInt32.logxor a b)
-  | BYTE -> (UInt8.logxor a b)
 
 
-let logand #t a b =
+
+let logand #t #l a b =
   match t with
   | U8 -> (UInt8.logand a b)
   | U16 -> (UInt16.logand a b)
   | U32 -> (UInt32.logand a b)
   | U64 -> (UInt64.logand a b)
   | U128 -> (UInt128.logand a b)
-  | SIZE -> (UInt32.logand a b)
-  | BYTE -> (UInt8.logand a b)
 
-let logor #t a b =
+
+let logor #t #l a b =
   match t with
   | U8 -> (UInt8.logor a b)
   | U16 -> (UInt16.logor a b)
   | U32 -> (UInt32.logor a b)
   | U64 -> (UInt64.logor a b)
   | U128 -> (UInt128.logor a b)
-  | SIZE -> (UInt32.logor a b)
-  | BYTE -> (UInt8.logor a b)
 
 
-let lognot #t a =
+
+let lognot #t #l a =
   match t with
   | U8 -> (UInt8.lognot a)
   | U16 -> (UInt16.lognot a)
   | U32 -> (UInt32.lognot a)
   | U64 -> (UInt64.lognot a)
   | U128 -> (UInt128.lognot a)
-  | SIZE -> (UInt32.lognot a)
-  | BYTE -> (UInt8.lognot a)
 
 
-let shift_right #t a b =
+
+let shift_right #t #l a b =
   match t with
   | U8 -> (UInt8.shift_right a b)
   | U16 -> (UInt16.shift_right a b)
   | U32 -> (UInt32.shift_right a b)
   | U64 -> (UInt64.shift_right a b)
   | U128 -> (UInt128.shift_right a b)
-  | SIZE -> (UInt32.shift_right a b)
-  | BYTE -> (UInt8.shift_right a b)
 
-let shift_left #t a b =
+
+let shift_left #t #l a b =
   match t with
   | U8 -> (UInt8.shift_left a b)
   | U16 -> (UInt16.shift_left a b)
   | U32 -> (UInt32.shift_left a b)
   | U64 -> (UInt64.shift_left a b)
   | U128 -> (UInt128.shift_left a b)
-  | SIZE -> (UInt32.shift_left a b)
-  | BYTE -> (UInt8.shift_left a b)
 
 
-let rotate_right #t a b =
-  (logor (shift_right a b)  (shift_left a (sub #SIZE (size (bits t)) b)))
 
-let rotate_left #t a b =
-  (logor (shift_left a b)  (shift_right a (sub #SIZE (size (bits t)) b)))
+let rotate_right #t #l a b =
+  (logor (shift_right a b)  (shift_left a (sub #U32 (size (bits t)) b)))
 
-let eq_mask #t a b =
+let rotate_left #t #l a b =
+  (logor (shift_left a b)  (shift_right a (sub #U32 (size (bits t)) b)))
+
+let eq_mask #t #l a b =
   match t with
   | U8 -> if FStar.UInt8.(a =^ b) then (u8 (maxint U8)) else (u8 0)
   | U16 -> if FStar.UInt16.(a =^ b) then (u16 (maxint U16)) else (u16 0)
   | U32 -> if FStar.UInt32.(a =^ b) then (u32 (maxint U32)) else (u32 0)
   | U64 -> if FStar.UInt64.(a =^ b) then (u64 (maxint U64)) else (u64 0)
   | U128 -> if FStar.UInt128.(a =^ b) then (u128 (maxint U128)) else (u128 0)
-  | SIZE -> if FStar.UInt32.(a =^ b) then (size_ (maxint U32)) else (size_ 0)
-  | BYTE -> if FStar.UInt8.(a =^ b) then (byte_ (maxint U8)) else (byte_ 0)
 
-let neq_mask #t a b =
+
+let neq_mask #t #l a b =
   match t with
   | U8 -> if not FStar.UInt8.(a =^ b) then (u8 (maxint U8)) else (u8 0)
   | U16 -> if not FStar.UInt16.(a =^ b) then (u16 (maxint U16)) else (u16 0)
   | U32 -> if not FStar.UInt32.(a =^ b) then (u32 (maxint U32)) else (u32 0)
   | U64 -> if not FStar.UInt64.(a =^ b) then (u64 (maxint U64)) else (u64 0)
   | U128 -> if not FStar.UInt128.(a =^ b) then (u128 (maxint U128)) else (u128 0)
-  | SIZE -> if not FStar.UInt32.(a =^ b) then (size_ (maxint U32)) else (size_ 0)
-  | BYTE -> if not FStar.UInt8.(a =^ b) then (byte_ (maxint U8)) else (byte_ 0)
 
-let gt_mask #t a b =
+
+let gt_mask #t #l a b =
   match t with
   | U8 -> if FStar.UInt8.(a >^ b) then (u8 (maxint U8)) else (u8 0)
   | U16 -> if FStar.UInt16.(a >^ b) then (u16 (maxint U16)) else (u16 0)
   | U32 -> if FStar.UInt32.(a >^ b) then (u32 (maxint U32)) else (u32 0)
   | U64 -> if FStar.UInt64.(a >^ b) then (u64 (maxint U64)) else (u64 0)
   | U128 -> if FStar.UInt128.(a >^ b) then (u128 (maxint U128)) else (u128 0)
-  | SIZE -> if FStar.UInt32.(a >^ b) then (size_ (maxint U32)) else (size_ 0)
-  | BYTE -> if FStar.UInt8.(a >^ b) then (byte_ (maxint U8)) else (byte_ 0)
 
-let gte_mask #t a b =
+
+let gte_mask #t #l a b =
   match t with
   | U8 -> if FStar.UInt8.(a >=^ b) then (u8 (maxint U8)) else (u8 0)
   | U16 -> if FStar.UInt16.(a >=^ b) then (u16 (maxint U16)) else (u16 0)
   | U32 -> if FStar.UInt32.(a >=^ b) then (u32 (maxint U32)) else (u32 0)
   | U64 -> if FStar.UInt64.(a >=^ b) then (u64 (maxint U64)) else (u64 0)
   | U128 -> if FStar.UInt128.(a >=^ b) then (u128 (maxint U128)) else (u128 0)
-  | SIZE -> if FStar.UInt32.(a >=^ b) then (size_ (maxint U32)) else (size_ 0)
-  | BYTE -> if FStar.UInt8.(a >=^ b) then (byte_ (maxint U8)) else (byte_ 0)
 
-let lt_mask #t a b =
+
+let lt_mask #t #l a b =
   match t with
   | U8 -> if FStar.UInt8.(a <^ b) then (u8 (maxint U8)) else (u8 0)
   | U16 -> if FStar.UInt16.(a <^ b) then (u16 (maxint U16)) else (u16 0)
   | U32 -> if FStar.UInt32.(a <^ b) then (u32 (maxint U32)) else (u32 0)
   | U64 -> if FStar.UInt64.(a <^ b) then (u64 (maxint U64)) else (u64 0)
   | U128 -> if FStar.UInt128.(a <^ b) then (u128 (maxint U128)) else (u128 0)
-  | SIZE -> if FStar.UInt32.(a <^ b) then (size_ (maxint U32)) else (size_ 0)
-  | BYTE -> if FStar.UInt8.(a <^ b) then (byte_ (maxint U8)) else (byte_ 0)
 
-let lte_mask #t a b =
+
+let lte_mask #t #l a b =
   match t with
   | U8 -> if FStar.UInt8.(a <=^ b) then (u8 (maxint U8)) else (u8 0)
   | U16 -> if FStar.UInt16.(a <=^ b) then (u16 (maxint U16)) else (u16 0)
   | U32 -> if FStar.UInt32.(a <=^ b) then (u32 (maxint U32)) else (u32 0)
   | U64 -> if FStar.UInt64.(a <=^ b) then (u64 (maxint U64)) else (u64 0)
   | U128 -> if FStar.UInt128.(a <=^ b) then (u128 (maxint U128)) else (u128 0)
-  | SIZE -> if FStar.UInt32.(a <=^ b) then (size_ (maxint U32)) else (size_ 0)
-  | BYTE -> if FStar.UInt8.(a <=^ b) then (byte_ (maxint U8)) else (byte_ 0)
 
-let eq_mask_lemma #t a b d = admit()
-let neq_mask_lemma #t a b d = admit()
-let gt_mask_lemma #t a b d = admit()
-let gte_mask_lemma #t a b d = admit()
-let lt_mask_lemma #t a b d = admit()
-let lte_mask_lemma #t a b d = admit()
+
+let eq_mask_lemma #t #l a b d = admit()
+let neq_mask_lemma #t #l a b d = admit()
+let gt_mask_lemma #t #l a b d = admit()
+let gte_mask_lemma #t #l a b d = admit()
+let lt_mask_lemma #t #l a b d = admit()
+let lte_mask_lemma #t #l a b d = admit()
 
 #set-options "--z3rlimit 10 --max_fuel 0 --max_ifuel 0"
 
 private
-val mod_mask_value: #t:inttype -> m:shiftval t -> Lemma
-  (uint_v (mod_mask #t m) == pow2 (uint_v m) - 1)
-let mod_mask_value #t m =
+val mod_mask_value: #t:inttype -> #l:secrecy_level -> m:shiftval t -> Lemma
+  (uint_v (mod_mask #t #l m) == pow2 (uint_v m) - 1)
+let mod_mask_value #t #l m =
   if uint_v m > 0 then
     begin
     let m = uint_v m in
@@ -376,8 +326,8 @@ let mod_mask_value #t m =
     UInt.shift_left_value_lemma #(bits t) 1 m
     end
 
-let mod_mask_lemma #t a m =
-  mod_mask_value #t m;
+let mod_mask_lemma #t #l a m =
+  mod_mask_value #t #l m;
   if uint_v m = 0 then
     UInt.logand_lemma_1 #(bits t) (uint_v a)
   else
@@ -391,41 +341,70 @@ let nat_mod_v #m x = x
 
 let div #t x y =
   match t with
-  | SIZE -> FStar.UInt32.div x y
-  | BYTE -> FStar.UInt8.div x y
+  | U8  -> (UInt8.div x y)
+  | U16 -> (UInt16.div x y)
+  | U32 -> (UInt32.div x y)
+  | U64 -> (UInt64.div x y)
 
 
 let mod #t x y =
   match t with
-  | SIZE -> FStar.UInt32.rem x y
-  | BYTE -> FStar.UInt8.rem x y
+  | U8  -> (UInt8.rem x y)
+  | U16 -> (UInt16.rem x y)
+  | U32 -> (UInt32.rem x y)
+  | U64 -> (UInt64.rem x y)
+
+
 
 let eq #t x y =
   match t with
-  | SIZE -> FStar.UInt32.eq x y
-  | BYTE -> FStar.UInt8.eq x y
+  | U8  -> (UInt8.eq x y)
+  | U16 -> (UInt16.eq x y)
+  | U32 -> (UInt32.eq x y)
+  | U64 -> (UInt64.eq x y)
+  | U128 -> (UInt128.eq x y)
+
 
 let ne #t x y =
   match t with
-  | SIZE -> not (FStar.UInt32.eq x y)
-  | BYTE -> not (FStar.UInt8.eq x y)
+  | U8  -> not (UInt8.eq x y)
+  | U16 -> not (UInt16.eq x y)
+  | U32 -> not (UInt32.eq x y)
+  | U64 -> not (UInt64.eq x y)
+  | U128 -> not (UInt128.eq x y)
 
 let lt #t x y =
   match t with
-  | SIZE -> FStar.UInt32.lt x y
-  | BYTE -> FStar.UInt8.lt x y
+  | U8  -> (UInt8.lt x y)
+  | U16 -> (UInt16.lt x y)
+  | U32 -> (UInt32.lt x y)
+  | U64 -> (UInt64.lt x y)
+  | U128 -> (UInt128.lt x y)
 
-let le #t x y =
+let lte #t x y =
   match t with
-  | SIZE -> FStar.UInt32.lte x y
-  | BYTE -> FStar.UInt8.lte x y
+  | U8  -> (UInt8.lte x y)
+  | U16 -> (UInt16.lte x y)
+  | U32 -> (UInt32.lte x y)
+  | U64 -> (UInt64.lte x y)
+  | U128 -> (UInt128.lte x y)
+
+
 
 let gt #t x y =
   match t with
-  | SIZE -> FStar.UInt32.gt x y
-  | BYTE -> FStar.UInt8.gt x y
+  | U8  -> (UInt8.gt x y)
+  | U16 -> (UInt16.gt x y)
+  | U32 -> (UInt32.gt x y)
+  | U64 -> (UInt64.gt x y)
+  | U128 -> (UInt128.gt x y)
 
-let ge #t x y =
+
+
+let gte #t x y =
   match t with
-  | SIZE -> FStar.UInt32.gte x y
-  | BYTE -> FStar.UInt8.gte x y
+  | U8  -> (UInt8.gte x y)
+  | U16 -> (UInt16.gte x y)
+  | U32 -> (UInt32.gte x y)
+  | U64 -> (UInt64.gte x y)
+  | U128 -> (UInt128.gte x y)
