lib/Lib.ByteSequence.fsti
@@ -18,9 +18,9 @@ let to_lbytes (b:bytes{length b > 0 /\ length b < max_size_t}) : lbytes (length 
 /// Conversions between natural numbers and sequences
 ///
 
-val nat_from_intseq_be: #t:inttype -> b:seq (uint_t t) -> Tot (n:nat{n < pow2 (length b * bits t)})
+val nat_from_intseq_be: #t:inttype -> #l:secrecy_level -> b:seq (uint_t t l) -> Tot (n:nat{n < pow2 (length b * bits t)})
 
-val nat_from_intseq_le: #t:inttype -> b:seq (uint_t t) -> Tot (n:nat{n < pow2 (length b * bits t)})
+val nat_from_intseq_le: #t:inttype -> #l:secrecy_level -> b:seq (uint_t t l) -> Tot (n:nat{n < pow2 (length b * bits t)})
 
 val nat_from_bytes_be: b:bytes -> Tot (n:nat{n < pow2 (length b * 8)})
 
@@ -30,25 +30,25 @@ val nat_to_bytes_be: len:nat -> n:nat{n < pow2 (8 * len)} ->  Tot (b:bytes{lengt
 
 val nat_to_bytes_le: len:nat -> n:nat{n < pow2 (8 * len)} ->  Tot (b:bytes{length b == len /\ n == nat_from_intseq_le #U8 b})
 
-val uint_to_bytes_le: #t:inttype -> u:uint_t t -> lbytes (numbytes t)
+val uint_to_bytes_le: #t:inttype -> #l:secrecy_level -> u:uint_t t l -> lbytes (numbytes t)
 
-val index_uint_to_bytes_le: #t:inttype -> u:uint_t t
+val index_uint_to_bytes_le: #t:inttype -> #l:secrecy_level -> u:uint_t t l
   -> Lemma
     (forall (i:nat{i < numbytes t}). index (uint_to_bytes_le u) i ==
                               u8 (uint_v u / pow2 (op_Multiply 8 i) % pow2 8))
-val uint_to_bytes_be: #t:inttype -> u:uint_t t -> lbytes (numbytes t)
+val uint_to_bytes_be: #t:inttype -> #l:secrecy_level -> u:uint_t t l -> lbytes (numbytes t)
 
-val uint_from_bytes_le: #t:inttype -> lbytes (numbytes t) -> u:uint_t t
+val uint_from_bytes_le: #t:inttype -> #l:secrecy_level -> lbytes (numbytes t) -> u:uint_t t l
 
-val uint_from_bytes_be: #t:inttype -> lbytes (numbytes t) -> u:uint_t t
+val uint_from_bytes_be: #t:inttype -> #l:secrecy_level -> lbytes (numbytes t) -> u:uint_t t l
 
-val uints_to_bytes_le: #t:inttype -> #len:size_nat{len * numbytes t < pow2 32} 
-  -> s:lseq (uint_t t) len -> b:lbytes (len * numbytes t)
-val uints_to_bytes_be: #t:inttype -> #len:size_nat{len * numbytes t < pow2 32}
-  -> s:lseq (uint_t t) len -> b:lbytes (len * numbytes t)
+val uints_to_bytes_le: #t:inttype -> #l:secrecy_level -> #len:size_nat{len * numbytes t < pow2 32} 
+  -> s:lseq (uint_t t l) len -> b:lbytes (len * numbytes t)
+val uints_to_bytes_be: #t:inttype -> #l:secrecy_level -> #len:size_nat{len * numbytes t < pow2 32}
+  -> s:lseq (uint_t t l) len -> b:lbytes (len * numbytes t)
 
 
-val uints_from_bytes_le: #t:inttype -> #len:size_nat{len * numbytes t < pow2 32} 
-  -> b:lbytes (len * numbytes t) -> s:lseq (uint_t t) len 
-val uints_from_bytes_be: #t:inttype -> #len:size_nat{len * numbytes t < pow2 32} 
-  -> b:lbytes (len * numbytes t) -> s:lseq (uint_t t) len 
+val uints_from_bytes_le: #t:inttype -> #l:secrecy_level -> #len:size_nat{len * numbytes t < pow2 32} 
+  -> b:lbytes (len * numbytes t) -> s:lseq (uint_t t l) len 
+val uints_from_bytes_be: #t:inttype -> #l:secrecy_level -> #len:size_nat{len * numbytes t < pow2 32} 
+  -> b:lbytes (len * numbytes t) -> s:lseq (uint_t t l) len 
