specs/tests/Spec.Salsa20.Test.fst
@@ -58,13 +58,13 @@ let test_column_round2 () =
 	 0x481c2027ul; 0x53a8e4b5ul; 0x4c1f89c5ul; 0x3f78c9c8ul])
 
 let test_salsa20_core () =
-  let st = uints_from_bytes_le #U32 #16 (of_list (List.Tot.map u8_from_UInt8
+  let st = uints_from_bytes_le #U32 #SEC #16 (of_list (List.Tot.map u8_from_UInt8
   [ 211uy;159uy; 13uy;115uy; 76uy; 55uy; 82uy;183uy; 3uy;117uy;222uy; 37uy;191uy;187uy;234uy;136uy;
 	 49uy;237uy;179uy; 48uy; 1uy;106uy;178uy;219uy;175uy;199uy;166uy; 48uy; 86uy; 16uy;179uy;207uy;
 	 31uy;240uy; 32uy; 63uy; 15uy; 83uy; 93uy;161uy;116uy;147uy; 48uy;113uy;238uy; 55uy;204uy; 36uy;
 	 79uy;201uy;235uy; 79uy; 3uy; 81uy;156uy; 47uy;203uy; 26uy;244uy;243uy; 88uy;118uy;104uy; 54uy])) in
   let st = salsa20_core st in
-  st = uints_from_bytes_le #U32 #16 (of_list (List.Tot.map u8_from_UInt8
+  st = uints_from_bytes_le #U32 #SEC #16 (of_list (List.Tot.map u8_from_UInt8
   [ 109uy; 42uy;178uy;168uy;156uy;240uy;248uy;238uy;168uy;196uy;190uy;203uy; 26uy;110uy;170uy;154uy;
 	 29uy; 29uy;150uy; 26uy;150uy; 30uy;235uy;249uy;190uy;163uy;251uy; 48uy; 69uy;144uy; 51uy; 57uy;
 	 118uy; 40uy;152uy;157uy;180uy; 57uy; 27uy; 94uy;107uy; 42uy;236uy; 35uy; 27uy;111uy;114uy;114uy;
